continuing to update BST proofs

concurrency/bst_conc_nblocking_spec.v
@@ -5,6 +5,7 @@ Require Import VST.atomics.general_locks.
 Require Import VST.atomics.SC_atomics.
 Require Import Coq.Sets.Ensembles.
 Require Import VST.msl.iter_sepcon.
+Require Import bst.puretree.
 Require Import bst.bst_conc_lemmas.
 Require Import bst.bst_conc_nblocking.
 
@@ -50,17 +51,17 @@ Program Definition insert_spec :=
   ATOMIC TYPE (rmaps.ConstType ( val * share * Z * val * globals*gname* gname)) OBJ BST INVS base.empty base.top
   WITH  b, sh, x, v, gv, g, g_root
   PRE [ (tptr atomic_ptr), tint, (tptr tvoid) ]
-          PROP (readable_share sh;Int.min_signed <= x <= Int.max_signed;  is_pointer_or_null v )
+          PROP (readable_share sh; Int.min_signed <= x <= Int.max_signed; is_pointer_or_null v)
           PARAMS (b; (Vint (Int.repr x)); v) GLOBALS(gv)
-          SEP  (mem_mgr gv; nodebox_rep sh b g_root g ) | (!!(sorted_tree BST)&&tree_rep g g_root b sh  BST )
+          SEP  (mem_mgr gv; nodebox_rep sh b g_root g) | (!!(sorted_tree BST) && tree_rep g g_root b sh BST)
   POST[ tvoid  ]
         PROP ()
         LOCAL ()
-       SEP (mem_mgr gv; nodebox_rep sh b g_root g) | (!!(sorted_tree (bst_conc_lemmas.insert x v BST)) && tree_rep g g_root  b sh (bst_conc_lemmas.insert x v BST) ). 
+       SEP (mem_mgr gv; nodebox_rep sh b g_root g) | (!!(sorted_tree (insert x v BST)) && tree_rep g g_root  b sh (insert x v BST)).
 
 Program Definition lookup_spec :=
   DECLARE _lookup
-  ATOMIC TYPE (rmaps.ConstType ( val * share* Z * globals * gname * gname))
+  ATOMIC TYPE (rmaps.ConstType (val * share* Z * globals * gname * gname))
          OBJ BST INVS base.empty base.top
   WITH b, sh, x, gv, g, g_root
   PRE [ (tptr atomic_ptr),tint]
@@ -73,7 +74,7 @@ Program Definition lookup_spec :=
     PROP ()
     LOCAL(temp ret_temp ret)
     SEP (mem_mgr gv; nodebox_rep sh b g_root g) |
-        (!! (sorted_tree BST /\ ret = (bst_conc_lemmas.lookup nullval x BST)) && tree_rep g g_root b sh BST).
+        (!! (sorted_tree BST /\ ret = lookup nullval x BST) && tree_rep g g_root b sh BST).
 
 Definition main_spec :=
  DECLARE _main
@@ -125,29 +126,32 @@ Qed.
    
 Lemma in_tree_split: forall g_in range p g, in_tree g_in range p g |-- in_tree g_in range p g * in_tree g_in range p g.
 Proof.
-intros. unfold in_tree. Intro sh. assert_PROP ( sh <> Share.bot).  { unfold ghost_part. sep_apply (own_valid (RA := ref_PCM (@ map_PCM gname range_info )) g ((Some (sh, ghosts.singleton  g_in (range, p)), None) ) compcert_rmaps.RML.R.NoneP). entailer!. inv H. simpl in H0. contradiction. } apply split_non_bot_share in H. destruct H as ( sh1 & sh2 & H1 & H2 & H).
-Exists sh1 sh2. rewrite <- (ghost_part_join (P := @ map_PCM gname range_info)  sh1 sh2 sh  (ghosts.singleton g_in (range, p))  (ghosts.singleton  g_in (range, p))).
-cancel. auto. { unfold sepalg.join. hnf. intro. hnf. simpl. destruct (ghosts.singleton  g_in (range, p) k). 
-  -  apply psepalg.lower_Some. unfold sepalg.join. hnf. split; hnf. rewrite merge_self;auto. split;auto.
-  - apply psepalg.lower_None1. 
-  } auto. auto. 
- Qed.
- 
-Definition node_data (info: option ghost_info) g  tp lp rp v (range:number * number)  :=  
-(match info with Some data =>  EX sh, !!(readable_share sh /\ Int.min_signed <= data.1.1.1 <= Int.max_signed/\ is_pointer_or_null lp /\ is_pointer_or_null rp /\ is_pointer_or_null data.1.1.2) && bst.bst_conc_nblocking_spec.atomic_ptr_at Ews v data.1.1.2 * malloc_token Ews t_struct_tree tp * data_at sh t_struct_tree (Vint (Int.repr data.1.1.1),(data.1.1.2,(lp,rp))) tp * in_tree  data.1.2 ( fst range, Finite_Integer (data.1.1.1)) lp g * in_tree data.2 ( Finite_Integer (data.1.1.1), snd range) rp g | None => !!(tp = nullval /\ lp = nullval /\ rp = nullval /\ v = nullval) && emp end).
+  intros. unfold in_tree. Intro sh.
+  assert_PROP (sh <> Share.bot). { unfold ghost_part. sep_apply (own_valid (RA := ref_PCM (@ map_PCM gname range_info )) g ((Some (sh, ghosts.singleton  g_in (range, p)), None) ) compcert_rmaps.RML.R.NoneP). entailer!. inv H. simpl in H0. contradiction. }
+  apply split_non_bot_share in H. destruct H as (sh1 & sh2 & H1 & H2 & H).
+  Exists sh1 sh2. rewrite <- (ghost_part_join (P := @ map_PCM gname range_info)  sh1 sh2 sh  (ghosts.singleton g_in (range, p))  (ghosts.singleton g_in (range, p))); auto.
+  hnf. intros k. destruct (ghosts.singleton g_in (range, p) k); constructor.
+  split; hnf; auto. symmetry; apply merge_id.
+Qed.
+
+Definition node_data (info: option ghost_info) g  tp lp rp v (r:range)  :=
+  match info with Some data =>
+    EX sh, !!(readable_share sh /\ Int.min_signed <= data.1.1.1 <= Int.max_signed /\ is_pointer_or_null lp /\ is_pointer_or_null rp /\ is_pointer_or_null data.1.1.2) &&
+      atomic_ptr_at Ews v data.1.1.2 * malloc_token Ews t_struct_tree tp * data_at sh t_struct_tree (Vint (Int.repr data.1.1.1),(data.1.1.2,(lp,rp))) tp * in_tree  data.1.2 (fst r, Finite_Integer (data.1.1.1)) lp g * in_tree data.2 (Finite_Integer (data.1.1.1), snd r) rp g
+  | None => !!(tp = nullval /\ lp = nullval /\ rp = nullval /\ v = nullval) && emp end.
 
 Definition node_information (info: option ghost_info) range g g_current tp lp rp v np  :=  bst.bst_conc_nblocking_spec.atomic_ptr_at Ews tp np * ghost_master1 (ORD := range_order)  (range, info) g_current * 
 node_data info g tp lp rp v range.
 
-Lemma node_data_R: forall (info: option ghost_info) g  tp lp rp v (range:number *number),  node_data info g tp  lp rp v range |-- if (eq_dec tp nullval) then !!(info = None /\ lp = nullval /\ rp = nullval /\ v = nullval) && emp  else 
-EX data, EX sh, !!(readable_share sh/\ info = Some data  /\ Int.min_signed <= data.1.1.1 <= Int.max_signed/\ is_pointer_or_null lp /\ is_pointer_or_null rp /\ is_pointer_or_null data.1.1.2) &&  bst.bst_conc_nblocking_spec.atomic_ptr_at Ews v data.1.1.2* malloc_token Ews t_struct_tree tp*  data_at sh t_struct_tree (Vint (Int.repr data.1.1.1),(data.1.1.2,(lp,rp))) tp * in_tree data.1.2( fst range, Finite_Integer data.1.1.1) lp g * in_tree data.2 ( Finite_Integer data.1.1.1, snd range) rp g.
+Lemma node_data_R: forall (info: option ghost_info) g  tp lp rp v (r:range),  node_data info g tp  lp rp v r |-- if (eq_dec tp nullval) then !!(info = None /\ lp = nullval /\ rp = nullval /\ v = nullval) && emp else 
+EX data, EX sh, !!(readable_share sh /\ info = Some data  /\ Int.min_signed <= data.1.1.1 <= Int.max_signed /\ is_pointer_or_null lp /\ is_pointer_or_null rp /\ is_pointer_or_null data.1.1.2) &&
+  atomic_ptr_at Ews v data.1.1.2 * malloc_token Ews t_struct_tree tp * data_at sh t_struct_tree (Vint (Int.repr data.1.1.1),(data.1.1.2,(lp,rp))) tp * in_tree data.1.2(fst r, Finite_Integer data.1.1.1) lp g * in_tree data.2 (Finite_Integer data.1.1.1, snd r) rp g.
 Proof.
-intros. unfold node_data.
-destruct info.
-- Intros sh.  assert_PROP (tp <> nullval).  { entailer!. } destruct (eq_dec tp nullval). contradiction. Exists g0 sh. entailer!.
-- Intros. destruct (eq_dec tp nullval). entailer!. contradiction.
+  intros. unfold node_data.
+  destruct info.
+  - Intros sh.  assert_PROP (tp <> nullval).  { entailer!. } destruct (eq_dec tp nullval). contradiction. Exists g0 sh. entailer!.
+  - Intros. destruct (eq_dec tp nullval). entailer!. contradiction.
 Qed.
-
 
 Lemma ghost_master1_alloc : forall r:node_info,
   emp |-- (|==> (EX g, ghost_master1 r g))%I.
@@ -164,7 +168,7 @@ Qed.
 
 
 Inductive range_info_in_tree (ri: node_info)
-          (range: number * number) (v :val) : ghost_tree -> Prop :=
+          (range: range) (v :val) : ghost_tree -> Prop :=
 | riit_none: (ri = (range, None)) /\ v = nullval -> range_info_in_tree ri range v E_ghost
 | riit_root: forall (l r: ghost_tree) (g1 g2: gname) (lp rp:val) k vp v',
     (ri = (range, Some (k, vp, g1, g2)) /\ v = v')  ->
@@ -177,7 +181,7 @@ Inductive range_info_in_tree (ri: node_info)
     range_info_in_tree ri range v (T_ghost l g1 lp k v' vp r g2 rp).
 
 
-Lemma extract_left_node_info_from_ghost_tree_rep:  forall  tg np b g_root g_current g (r_root: number * number) (range:number*number),
+Lemma extract_left_node_info_from_ghost_tree_rep:  forall  tg np b g_root g_current g (r_root: range) (range:number*number),
    (find_ghost_set tg g_root r_root b) g_current = Some (range,np) -> ghost_tree_rep tg b g_root g r_root  |--  EX tp:val,  EX o:option ghost_info, EX lp:val, EX rp:val, EX v:val, 
    !! range_info_in_tree (range,o) r_root v tg &&  node_information o range g g_current tp  lp rp v np  *
    ( node_information o range g g_current tp  lp rp v np  -* ghost_tree_rep tg b g_root g r_root).
@@ -206,7 +210,7 @@ Qed.
 
 Lemma range_info_in_tree_In: forall tg x vp ga gb range v r_root,
     range_info_in_tree (range,  Some (x, vp, ga, gb)) r_root v tg ->
-   bst.bst_conc_lemmas.In x (find_pure_tree tg).
+   In x (find_pure_tree tg).
 Proof.
   intros. revert tg range r_root H. induction tg; intros;inversion H; inversion H0;
   simpl. inv H1.
@@ -215,10 +219,10 @@ Proof.
   - apply InRight. eapply IHtg2; eauto.
 Qed.
 
-Lemma sorted_tree_look_up_in: forall x v vp ga gb tg range r_root,
+Lemma sorted_tree_lookup_in: forall x v vp ga gb tg range r_root,
     sorted_tree (find_pure_tree tg) ->
     range_info_in_tree (range, Some (x, vp, ga, gb)) r_root v tg ->
-    bst.bst_conc_lemmas.lookup nullval x (find_pure_tree tg) = v.
+    lookup nullval x (find_pure_tree tg) = v.
 Proof.
   intros. revert tg range r_root H H0. induction tg; intros;
   inversion H0; inversion H1. inv H. simpl. auto.
@@ -232,8 +236,8 @@ Proof.
     intros. assert (x <? k = false) by (rewrite Z.ltb_ge; lia). now rewrite H1.
 Qed.
 
-Lemma range_info_in_tree_IsEmptyNode: forall ri range tg,
-    range_info_in_tree (ri, None) range nullval tg -> IsEmptyNode ri (find_pure_tree tg) range.
+Lemma range_info_in_tree_EmptyRange: forall ri range tg,
+    range_info_in_tree (ri, None) range nullval tg -> EmptyRange ri (find_pure_tree tg) range.
 Proof.
   intros. destruct range as [l r]. revert tg l r H.
   induction tg; intros; inv H; simpl in *.
@@ -244,52 +248,52 @@ Proof.
 Qed.
 
 Lemma range_info_in_tree_not_In: forall tg x range r_root,
-    sorted_tree (find_pure_tree tg) -> check_key_exist' x range = true ->
-    (forall k : key,  bst.bst_conc_lemmas.In k (find_pure_tree tg) -> check_key_exist' k r_root = true) ->
-    range_info_in_tree (range, None) r_root nullval tg -> ~  bst.bst_conc_lemmas.In x (find_pure_tree tg).
+    sorted_tree (find_pure_tree tg) -> key_in_range x range = true ->
+    (forall k : key,  In k (find_pure_tree tg) -> key_in_range k r_root = true) ->
+    range_info_in_tree (range, None) r_root nullval tg -> ~In x (find_pure_tree tg).
 Proof.
   intros. revert tg r_root H H1 H2. induction tg; intros; simpl in *.
   1: intro; inv H3. inv H. inv H2. 1: inv H3. inv H.
-  - assert (forall y : key,  bst.bst_conc_lemmas.In y (find_pure_tree tg1) ->
-                            check_key_exist' y (r_root.1, Finite_Integer k) = true). {
+  - assert (forall y : key,  In y (find_pure_tree tg1) ->
+                            key_in_range y (r_root.1, Finite_Integer k) = true). {
       intros. rewrite andb_true_iff. split.
-      - assert (check_key_exist' y r_root = true) by now apply H1, InLeft.
+      - assert (key_in_range y r_root = true) by now apply H1, InLeft.
         destruct r_root as [r1 r2]. simpl. apply andb_true_iff in H2.
         now destruct H3.
       - red in H9. simpl. specialize (H9 _ H). rewrite Z.ltb_lt. lia. }
-    assert (range_inclusion range (r_root.1, Finite_Integer k) = true). {
+    assert (range_incl range (r_root.1, Finite_Integer k) = true). {
         eapply range_inside_range with (t := find_pure_tree tg1); auto.
-        now apply range_info_in_tree_IsEmptyNode. } destruct range as [r1 r2].
+        now apply range_info_in_tree_EmptyRange. } destruct range as [r1 r2].
      apply andb_true_iff in H2. destruct H2.
     apply andb_true_iff in H0. destruct H0. specialize (IHtg1 _ H7 H H3).
     intro. inv H6; auto.
     + assert (less_than (Finite_Integer k) (Finite_Integer k) = true) by
-          (eapply less_than_less_than_equal_transitivity; eauto).
+          (eapply less_than_less_than_equal_trans; eauto).
       rewrite less_than_irrefl in H6. inv H6.
     + assert (less_than (Finite_Integer x) (Finite_Integer k) = true) by
-          (eapply less_than_less_than_equal_transitivity; eauto). simpl in H6.
+          (eapply less_than_less_than_equal_trans; eauto). simpl in H6.
       apply Z.ltb_lt in H6. specialize (H10 _ H12). lia.
-  - assert (forall y : key, bst.bst_conc_lemmas.In y (find_pure_tree tg2) ->
-                            check_key_exist' y (Finite_Integer k, r_root.2) = true). {
+  - assert (forall y : key, In y (find_pure_tree tg2) ->
+                            key_in_range y (Finite_Integer k, r_root.2) = true). {
       intros. rewrite andb_true_iff. split.
       - red in H10. simpl. specialize (H10 _ H). now rewrite Z.ltb_lt.
-      - assert (check_key_exist' y r_root = true) by now apply H1, InRight.
+      - assert (key_in_range y r_root = true) by now apply H1, InRight.
         destruct r_root as [r1 r2]. simpl. apply andb_true_iff in H2.
         now destruct H2. }
-    assert (range_inclusion range (Finite_Integer k, r_root.2) = true). {
+    assert (range_incl range (Finite_Integer k, r_root.2) = true). {
         eapply range_inside_range with (t := find_pure_tree tg2); auto.
-        now apply range_info_in_tree_IsEmptyNode. } destruct range as [r1 r2].
+        now apply range_info_in_tree_EmptyRange. } destruct range as [r1 r2].
     apply andb_true_iff in H2. destruct H2. apply andb_true_iff in H0. destruct H0.
     specialize (IHtg2 _ H8 H H3). intro. inv H6; auto.
     + assert (less_than (Finite_Integer k) (Finite_Integer k) = true) by
-          (eapply less_than_equal_less_than_transitivity; eauto).
+          (eapply less_than_equal_less_than_trans; eauto).
       rewrite less_than_irrefl in H6. inv H6.
     + assert (less_than (Finite_Integer k) (Finite_Integer x) = true) by
-          (eapply less_than_equal_less_than_transitivity; eauto).
+          (eapply less_than_equal_less_than_trans; eauto).
       simpl in H6. apply Z.ltb_lt in H6. specialize (H9 _ H12). lia.
 Qed.
 
-Lemma lookup_not_in: forall t x, ~ bst.bst_conc_lemmas.In x t -> bst.bst_conc_lemmas.lookup nullval x t = nullval.
+Lemma lookup_not_in: forall t x, ~ In x t -> lookup nullval x t = nullval.
 Proof.
   intros. revert t H. induction t; intros; simpl; auto. destruct (x <? k) eqn: ?.
   - apply IHt1. intro. now apply H, InLeft.
@@ -300,16 +304,15 @@ Proof.
 Qed.
 
 
-
-Lemma extract_node_info_from_ghost_tree_rep_2:  forall  tg np b g_root x v  g_current g (r_root: number * number) n n0, 
-  (find_ghost_set tg g_root r_root b) g_current = Some (n,n0,np)-> (forall k, In_ghost k tg -> check_key_exist' k r_root = true) -> sorted_ghost_tree tg-> ghost_tree_rep tg b g_root g r_root  |--  EX tp:val,  EX o:option ghost_info, EX lp:val, EX rp:val, EX v0:val,
-     !!(range_inclusion (n,n0) r_root = true ) && node_information o (n, n0) g g_current tp lp rp v0 np  *
+Lemma extract_node_info_from_ghost_tree_rep_2:  forall  tg np b g_root x v  g_current g (r_root: range) n n0,
+  (find_ghost_set tg g_root r_root b) g_current = Some (n,n0,np)-> (forall k, In_ghost k tg -> key_in_range k r_root = true) -> sorted_ghost_tree tg-> ghost_tree_rep tg b g_root g r_root  |--  EX tp:val,  EX o:option ghost_info, EX lp:val, EX rp:val, EX v0:val,
+     !!(range_incl (n,n0) r_root = true ) && node_information o (n, n0) g g_current tp lp rp v0 np  *
       (( node_information o (n, n0) g g_current tp lp rp v0 np  -* ghost_tree_rep tg b g_root g r_root)
-    && (ALL g1 g2:gname,ALL tp1:val, ALL lp1:val, ALL rp1:val, ALL vp:val, ( !!(o = None /\ tp = nullval /\ lp = nullval /\ rp = nullval /\ (check_key_exist' x (n,n0) = true) ) &&
+    && (ALL g1 g2:gname,ALL tp1:val, ALL lp1:val, ALL rp1:val, ALL vp:val, (!!(o = None /\ tp = nullval /\ lp = nullval /\ rp = nullval /\ (key_in_range x (n,n0) = true) ) &&
         node_information (Some (x,vp,g1,g2)) (n, n0) g g_current tp1 lp1 rp1 v np * node_information None (n, Finite_Integer x) g g1 nullval nullval nullval nullval lp1 * 
         node_information None (Finite_Integer x, n0) g g2 nullval nullval nullval nullval rp1)  -* (!! IsEmptyGhostNode (n,n0,o) tg r_root && ghost_tree_rep (insert_ghost x v vp tg g1 lp1 g2 rp1 ) b g_root g r_root))
-    && (ALL g1 g2:gname, ALL (vp:val), ( !!(o = Some(x,vp,g1,g2) /\ (check_key_exist' x (n,n0) = true)) && node_information (Some (x,vp,g1,g2)) (n, n0) g g_current tp lp rp v np  )
-        -* ( !! In_ghost x tg &&ghost_tree_rep (insert_ghost x v vp tg g1 lp g2 rp ) b g_root g r_root)) ).
+    && (ALL g1 g2:gname, ALL (vp:val), (!!(o = Some(x,vp,g1,g2) /\ (key_in_range x (n,n0) = true)) && node_information (Some (x,vp,g1,g2)) (n, n0) g g_current tp lp rp v np  )
+        -* (!! In_ghost x tg &&ghost_tree_rep (insert_ghost x v vp tg g1 lp g2 rp ) b g_root g r_root))).
 Proof.
 intros. 
 revert dependent r_root. 
@@ -317,13 +320,13 @@ revert dependent b.
 revert dependent g_root.
 induction tg.
  - intros. destruct r_root. simpl in H. unfold ghosts.singleton in H.  destruct (eq_dec g_current g_root). inv H. Exists nullval (@None ghost_info) nullval nullval nullval. unfold node_information at 1, node_data at 1. simpl. entailer!.
-  { rewrite less_than_equal_itself. rewrite less_than_equal_itself. repeat (split;auto). } repeat apply andp_right.
+  { rewrite less_than_equal_refl. rewrite less_than_equal_refl. repeat (split;auto). } repeat apply andp_right.
     * unfold node_information, node_data;simpl. entailer!. rewrite prop_true_andp. apply wand_refl_cancel_right. auto.
     *  apply allp_right; intro g1. apply allp_right;intro g2. apply allp_right;intro tp1.  apply allp_right;intro lp1.  apply allp_right;intro rp1. apply allp_right;intro vp. rewrite <- wand_sepcon_adjoint. unfold node_information, node_data;simpl. Intro sh.  rewrite <-!sepcon_assoc. Exists tp1 sh. cancel. entailer!. apply InEmptyGhostTree;auto.
     *  apply allp_right; intro g1. apply allp_right;intro g2. apply allp_right;intro vp.  rewrite <- wand_sepcon_adjoint. Intros. discriminate. 
     * discriminate.
  - intros.  simpl in H. unfold map_upd in H. destruct (eq_dec g_current g_root) eqn: Eqn.
-   * inv H. simpl. Intros tp sh.  Exists  tp (Some (k, v2, g0, g1)) v0 v3 v1.  unfold node_information at 1, node_data at 1. Exists sh. entailer!. repeat rewrite less_than_equal_itself. simpl;auto. cancel.  repeat  apply andp_right.
+   * inv H. simpl. Intros tp sh.  Exists  tp (Some (k, v2, g0, g1)) v0 v3 v1.  unfold node_information at 1, node_data at 1. Exists sh. entailer!. repeat rewrite less_than_equal_refl. simpl;auto. cancel.  repeat  apply andp_right.
      +   rewrite <- wand_sepcon_adjoint. unfold node_information, node_data. simpl.  Intro sh1. Exists  tp sh1. entailer!.
      + apply allp_right; intro g2. apply allp_right;intro g3. apply allp_right;intro tp1. apply allp_right;intro lp1.  apply allp_right;intro rp1.  apply allp_right;intro vp.  rewrite <- wand_sepcon_adjoint. Intros;discriminate.
      + apply allp_right; intro g2. apply allp_right;intro g3. apply allp_right;intro vp. rewrite <- wand_sepcon_adjoint. assert_PROP (Some (k, v2, g0, g1) = Some (x, vp, g2, g3)). { entailer!. } inv H6;subst. simpl.
@@ -331,10 +334,10 @@ induction tg.
  * unfold map_add in H. rename n1 into eq. destruct r_root as [n1 n2]. simpl in H. remember (find_ghost_set tg1 g0 (n1, Finite_Integer k) v0 g_current) as left_set. destruct left_set.  rename g2 into g_left.
     ** simpl.  Intros tp sh. destruct (x <? k) eqn: E1.
         + simpl. inv H1.  sep_apply IHtg1. rewrite <- Heqleft_set;apply H.
-         {  intros. assert (check_key_exist' k0 (n1, n2) = true). { apply H0. apply InLeft_ghost. apply H1. } unfold check_key_exist' in * . apply andb_prop in H4. destruct H4.
+         {  intros. assert (key_in_range k0 (n1, n2) = true). { apply H0. apply InLeft_ghost. apply H1. } unfold key_in_range in * . apply andb_prop in H4. destruct H4.
              unfold gt_ghost in H15. apply H15 in H1. rewrite H4;simpl. apply Zaux.Zlt_bool_true. lia. }
              rewrite sepcon_comm. Intros  tp0 o lp rp v4. Exists tp0 o lp rp v4. entailer!. 
-            { simpl in H1.  apply andb_prop in H1. destruct H1. assert (check_key_exist' k (n1, n2) = true). { apply H0. apply InRoot_ghost. auto. } unfold check_key_exist' in H9.  apply andb_prop in H9. destruct H9. rewrite H1;simpl. apply less_than_to_less_than_equal in H10. apply less_than_equal_transitivity with (b := (Finite_Integer k) ). apply H7. apply H10. }
+            { simpl in H1.  apply andb_prop in H1. destruct H1. assert (key_in_range k (n1, n2) = true). { apply H0. apply InRoot_ghost. auto. } unfold key_in_range in H9.  apply andb_prop in H9. destruct H9. rewrite H1;simpl. apply less_than_to_less_than_equal in H10. apply less_than_equal_trans with (b := (Finite_Integer k) ). apply H7. apply H10. }
              rewrite distrib_sepcon_andp.  rewrite distrib_sepcon_andp.  repeat apply andp_derives.
           ++ rewrite <- ( emp_wand (bst_conc_nblocking_spec.atomic_ptr_at Ews tp b * _ * _ * _ * _* _ * _ * _)). rewrite wand_sepcon_wand. apply wand_derives. cancel. Exists tp sh. entailer!.
           ++ apply allp_right; intro g2. apply allp_right;intro g3. apply allp_right;intro tp1. apply allp_right;intro lp1.  apply allp_right;intro rp1. apply allp_right;intro vp. repeat (rewrite allp_sepcon2; eapply allp_left). instantiate(1:= rp1). instantiate(1:= g3). instantiate(1:= lp1).   instantiate(1:= g2).  instantiate(1:= vp). instantiate (1:= tp1).  rewrite <- ( emp_wand (bst_conc_nblocking_spec.atomic_ptr_at Ews tp b * _ * _ * _ * _* _ * _* _)).
@@ -342,42 +345,42 @@ induction tg.
           ++ apply allp_right; intro g2. apply allp_right;intro g3. apply allp_right;intro vp. repeat (rewrite allp_sepcon2; eapply allp_left). instantiate(1:= g3).  instantiate(1:= g2).  instantiate(1:= vp).  rewrite <- ( emp_wand (bst_conc_nblocking_spec.atomic_ptr_at Ews tp b * _ * _ * _ * _* _*_*_)).
              rewrite wand_sepcon_wand. apply wand_derives. cancel. simpl. Exists tp sh. entailer!. apply InLeft_ghost. apply H7. 
        +  simpl. inv H1. sep_apply IHtg1.  rewrite <- Heqleft_set;apply H.
-            { intros. assert (check_key_exist' k0 (n1, n2) = true). { apply H0. apply InLeft_ghost. apply H1. } unfold check_key_exist' in * . apply andb_prop in H4. destruct H4.
+            { intros. assert (key_in_range k0 (n1, n2) = true). { apply H0. apply InLeft_ghost. apply H1. } unfold key_in_range in * . apply andb_prop in H4. destruct H4.
              unfold gt_ghost in H15. apply H15 in H1. rewrite H4;simpl. apply Zaux.Zlt_bool_true. lia. }  
          Intros tp0 o lp rp v4. Exists  tp0 o lp rp v4. entailer!.
-         { simpl in H1.  apply andb_prop in H1. destruct H1. assert (check_key_exist' k (n1, n2) = true). { apply H0. apply InRoot_ghost. auto. } unfold check_key_exist' in H9.  apply andb_prop in H9. destruct H9. rewrite H1;simpl. apply less_than_to_less_than_equal in H10. apply less_than_equal_transitivity with (b := (Finite_Integer k) ). apply H7. apply H10. }
+         { simpl in H1.  apply andb_prop in H1. destruct H1. assert (key_in_range k (n1, n2) = true). { apply H0. apply InRoot_ghost. auto. } unfold key_in_range in H9.  apply andb_prop in H9. destruct H9. rewrite H1;simpl. apply less_than_to_less_than_equal in H10. apply less_than_equal_trans with (b := (Finite_Integer k) ). apply H7. apply H10. }
               rewrite -> 7sepcon_assoc, sepcon_comm.  rewrite distrib_sepcon_andp.  rewrite distrib_sepcon_andp.  repeat  apply andp_derives.
          ++  rewrite <- !sepcon_assoc. rewrite <- ( emp_wand (bst_conc_nblocking_spec.atomic_ptr_at Ews tp b * _ * _ * _ * _* _ * _ * _)). rewrite wand_sepcon_wand. apply wand_derives. cancel. Exists tp sh. entailer!.
          ++ apply allp_right; intro g2. apply allp_right;intro g3. apply allp_right;intro tp1. apply allp_right;intro lp1.  apply allp_right;intro rp1. apply allp_right;intro vp.  repeat (rewrite allp_sepcon2; eapply allp_left). instantiate(1:= rp1). instantiate(1:= g3). instantiate(1:= lp1). instantiate(1:= g2).  instantiate(1:= vp).  instantiate(1:= tp1). 
-              rewrite <- wand_sepcon_adjoint. assert_PROP (check_key_exist' x (n,n0) = true). { simpl. entailer!. } 
+              rewrite <- wand_sepcon_adjoint. assert_PROP (key_in_range x (n,n0) = true). { simpl. entailer!. } 
               assert (x < k). { simpl in H1. apply andb_prop in H1. apply andb_prop in H7.  destruct H1,H7. unfold less_than_equal, less_than in *. destruct n0.  apply Z.ltb_lt in H10. apply Zle_bool_imp_le in H9. lia. discriminate. discriminate.  } 
               apply Z.ltb_nlt in E1. lia. 
          ++ apply allp_right; intro g2. apply allp_right;intro g3. apply allp_right;intro vp. repeat (rewrite allp_sepcon2; eapply allp_left). instantiate(1:= g2).  instantiate(1:= g3).  instantiate(1:= vp). 
-              rewrite <- wand_sepcon_adjoint. assert_PROP (check_key_exist' x (n,n0) = true). { simpl. entailer!. } 
+              rewrite <- wand_sepcon_adjoint. assert_PROP (key_in_range x (n,n0) = true). { simpl. entailer!. } 
               assert (x < k). { simpl in H1. apply andb_prop in H7. apply andb_prop in H1.  destruct H1,H7. unfold less_than_equal, less_than in *. destruct n0.  apply Z.ltb_lt in H10. apply Zle_bool_imp_le in H9. lia. discriminate. discriminate.  } 
              apply Z.ltb_nlt in E1. lia. 
   ** simpl. Intros tp sh. destruct (x <? k) eqn: E1.
        + simpl. inv H1.  unfold lt_ghost in H14. sep_apply IHtg2.
-         { intros. assert (check_key_exist' k0 (n1, n2) = true). { apply H0. apply InRight_ghost. apply H1. } unfold check_key_exist' in * . apply andb_prop in H4. destruct H4.
+         { intros. assert (key_in_range k0 (n1, n2) = true). { apply H0. apply InRight_ghost. apply H1. } unfold key_in_range in * . apply andb_prop in H4. destruct H4.
          apply H16 in H1. rewrite H5;simpl. rewrite andb_comm;simpl. apply Zaux.Zlt_bool_true. lia. }       
        Intros tp0 o lp rp v4. Exists tp0 o lp rp v4. entailer!. 
-         { simpl in H1.  apply andb_prop in H1. destruct H1. assert (check_key_exist' k (n1, n2) = true). { apply H0. apply InRoot_ghost. auto. } unfold check_key_exist' in H9.  apply andb_prop in H9. destruct H9. rewrite H7;simpl. rewrite andb_comm;simpl. apply less_than_to_less_than_equal in H9. apply less_than_equal_transitivity with (b := (Finite_Integer k) ). apply H9. apply H1. }
+         { simpl in H1.  apply andb_prop in H1. destruct H1. assert (key_in_range k (n1, n2) = true). { apply H0. apply InRoot_ghost. auto. } unfold key_in_range in H9.  apply andb_prop in H9. destruct H9. rewrite H7;simpl. rewrite andb_comm;simpl. apply less_than_to_less_than_equal in H9. apply less_than_equal_trans with (b := (Finite_Integer k) ). apply H9. apply H1. }
           rewrite -> 7sepcon_assoc, sepcon_comm.  rewrite distrib_sepcon_andp.  rewrite distrib_sepcon_andp.  repeat  apply andp_derives.
          ++  rewrite <- !sepcon_assoc. rewrite <- ( emp_wand (bst_conc_nblocking_spec.atomic_ptr_at Ews tp b * _ * _ * _ * _* _ * _*_)). rewrite wand_sepcon_wand. apply wand_derives. cancel. Exists tp sh. entailer!.
          ++ apply allp_right; intro g2. apply allp_right;intro g3. apply allp_right;intro tp1. apply allp_right;intro lp1.  apply allp_right;intro rp1. apply allp_right;intro vp.  repeat (rewrite allp_sepcon2; eapply allp_left). instantiate(1:= rp1). instantiate(1:= g3). instantiate(1:= lp1).   instantiate(1:= g2). instantiate(1:= vp).  instantiate (1:= tp1).
-              rewrite <- wand_sepcon_adjoint. assert_PROP (check_key_exist' x (n,n0) = true). { simpl. entailer!. }  
+              rewrite <- wand_sepcon_adjoint. assert_PROP (key_in_range x (n,n0) = true). { simpl. entailer!. }  
               assert (k < x). { simpl in H1. apply andb_prop in H7. apply andb_prop in H1.  destruct H1,H7. unfold less_than_equal, less_than in *. destruct n.  apply Zle_bool_imp_le in H1. apply Z.ltb_lt in H7. lia. discriminate. discriminate.  } 
              apply Z.ltb_lt in E1. lia. 
          ++ apply allp_right; intro g2. apply allp_right;intro g3. apply allp_right;intro vp0. repeat (rewrite allp_sepcon2; eapply allp_left). instantiate(1:= g2).  instantiate(1:= g3). instantiate(1:= vp0). 
-              rewrite <- wand_sepcon_adjoint. assert_PROP (check_key_exist' x (n,n0) = true). { simpl. entailer!. }  
+              rewrite <- wand_sepcon_adjoint. assert_PROP (key_in_range x (n,n0) = true). { simpl. entailer!. }  
               assert (k < x). { simpl in H1. apply andb_prop in H7. apply andb_prop in H1.  destruct H1,H7. unfold less_than_equal, less_than in *. destruct n.  apply Zle_bool_imp_le in H1. apply Z.ltb_lt in H7. lia. discriminate. discriminate.  } 
               apply Z.ltb_lt in E1. lia.  
         + destruct (k <? x) eqn:E2. simpl;inv H1.  
           ++ sep_apply IHtg2.
-            {  intros. assert (check_key_exist' k0 (n1, n2) = true). { apply H0. apply InRight_ghost. apply H1. } unfold check_key_exist' in * . apply andb_prop in H4. destruct H4.
+            {  intros. assert (key_in_range k0 (n1, n2) = true). { apply H0. apply InRight_ghost. apply H1. } unfold key_in_range in * . apply andb_prop in H4. destruct H4.
                 apply H16 in H1. rewrite H5;simpl. rewrite andb_comm;simpl. apply Zaux.Zlt_bool_true. lia. }
             Intros tp0 o lp rp v4. Exists  tp0 o lp rp v4. entailer!.
-            { simpl in H1.  apply andb_prop in H1. destruct H1. assert (check_key_exist' k (n1, n2) = true). { apply H0. apply InRoot_ghost. auto. } unfold check_key_exist' in H6.  apply andb_prop in H9. destruct H9. rewrite H7;simpl. rewrite andb_comm;simpl.  apply less_than_to_less_than_equal in H9. apply less_than_equal_transitivity with (b := (Finite_Integer k) ). apply H9. apply H1. }
+            { simpl in H1.  apply andb_prop in H1. destruct H1. assert (key_in_range k (n1, n2) = true). { apply H0. apply InRoot_ghost. auto. } unfold key_in_range in H6.  apply andb_prop in H9. destruct H9. rewrite H7;simpl. rewrite andb_comm;simpl.  apply less_than_to_less_than_equal in H9. apply less_than_equal_trans with (b := (Finite_Integer k) ). apply H9. apply H1. }
            rewrite -> 7sepcon_assoc, sepcon_comm.  rewrite distrib_sepcon_andp.  rewrite distrib_sepcon_andp.  repeat apply andp_derives.
             +++  rewrite <- !sepcon_assoc.  rewrite <- ( emp_wand (bst_conc_nblocking_spec.atomic_ptr_at Ews tp b * _ * _ * _ * _* _ * _*_)). rewrite wand_sepcon_wand. apply wand_derives. cancel. Exists tp sh. entailer!.
             +++  apply allp_right; intro g2. apply allp_right;intro g3. apply allp_right;intro tp1. apply allp_right;intro lp1.  apply allp_right;intro rp1. apply allp_right;intro vp. repeat (rewrite allp_sepcon2; eapply allp_left). instantiate(1:= rp1). instantiate(1:= g3). instantiate(1:= lp1). instantiate(1:= g2). instantiate (1 := vp).  instantiate(1:= tp1). rewrite <- !sepcon_assoc.   rewrite <- ( emp_wand (bst_conc_nblocking_spec.atomic_ptr_at Ews tp b * _ * _ * _ * _* _ * _*_)).
@@ -385,21 +388,19 @@ induction tg.
             +++ apply allp_right; intro g2. apply allp_right;intro g3. apply allp_right;intro v5. repeat (rewrite allp_sepcon2; eapply allp_left). instantiate(1:= g3).  instantiate(1:= g2).  instantiate(1:= v5). rewrite <- !sepcon_assoc.  rewrite <- ( emp_wand (bst_conc_nblocking_spec.atomic_ptr_at Ews tp b * _ * _ * _ * _* _ *_*_)).
              rewrite wand_sepcon_wand. apply wand_derives. cancel. simpl. Exists tp sh. entailer!. apply InRight_ghost. apply H7. 
          ++   inv H1.  assert (k = x ). { apply Z.ltb_nlt in E1. apply Z.ltb_nlt in E2. lia. } sep_apply IHtg2. 
-            { intros. assert (check_key_exist' k0 (n1, n2) = true). { apply H0. apply InRight_ghost. apply H4. } unfold check_key_exist' in * . apply andb_prop in H5. destruct H5.
+            { intros. assert (key_in_range k0 (n1, n2) = true). { apply H0. apply InRight_ghost. apply H4. } unfold key_in_range in * . apply andb_prop in H5. destruct H5.
                apply H16 in H4. rewrite H6;simpl. rewrite andb_comm;simpl. apply Zaux.Zlt_bool_true. lia. }
             Intros  tp0 o lp rp v4. Exists  tp0 o lp rp v4. entailer!. 
-            { simpl in H3.  apply andb_prop in H4. destruct H4. assert (check_key_exist' x (n1, n2) = true). { apply H0. apply InRoot_ghost. auto. } unfold check_key_exist' in H9.  apply andb_prop in H9. destruct H9. rewrite H4;simpl. rewrite andb_comm;simpl. apply less_than_to_less_than_equal in H9. apply less_than_equal_transitivity with (b := (Finite_Integer x) ). apply H9. apply H1. }
+            { simpl in H3.  apply andb_prop in H4. destruct H4. assert (key_in_range x (n1, n2) = true). { apply H0. apply InRoot_ghost. auto. } unfold key_in_range in H9.  apply andb_prop in H9. destruct H9. rewrite H4;simpl. rewrite andb_comm;simpl. apply less_than_to_less_than_equal in H9. apply less_than_equal_trans with (b := (Finite_Integer x) ). apply H9. apply H1. }
              rewrite -> 7sepcon_assoc, sepcon_comm.  rewrite distrib_sepcon_andp.  rewrite distrib_sepcon_andp.  repeat  apply andp_derives.
             +++  rewrite <- !sepcon_assoc.  rewrite <- ( emp_wand (bst_conc_nblocking_spec.atomic_ptr_at Ews tp b * _ * _ * _ * _* _ * _*_)). rewrite wand_sepcon_wand. apply wand_derives. cancel. Exists tp sh. entailer!.
             +++ apply allp_right; intro g2. apply allp_right;intro g3. apply allp_right;intro tp1. apply allp_right;intro lp1.  apply allp_right;intro rp1. apply allp_right;intro vp. repeat (rewrite allp_sepcon2; eapply allp_left). instantiate(1:= rp1). instantiate(1:= g3). instantiate(1:= lp1).  instantiate(1:= g2). instantiate(1:= vp).  instantiate(1:= tp1). 
-                   rewrite <- wand_sepcon_adjoint. assert_PROP (check_key_exist' x (n,n0) = true). { simpl. entailer!. } 
+                   rewrite <- wand_sepcon_adjoint. assert_PROP (key_in_range x (n,n0) = true). { simpl. entailer!. } 
                    simpl in H2.  apply andb_prop in H4. apply andb_prop in H1.  destruct H4, H1. destruct n. simpl in H1. apply Z.ltb_lt in H1. apply Zle_bool_imp_le in H4. lia. discriminate. simpl in H1. discriminate. 
         
             +++ apply allp_right; intro g2. apply allp_right;intro g3. apply allp_right;intro v5. repeat (rewrite allp_sepcon2; eapply allp_left). instantiate(1:= g2).  instantiate(1:= g3).  instantiate(1:= v5). 
-                  rewrite <- wand_sepcon_adjoint. assert_PROP (check_key_exist' x (n, n0) = true). { simpl. entailer!. } 
+                  rewrite <- wand_sepcon_adjoint. assert_PROP (key_in_range x (n, n0) = true). { simpl. entailer!. } 
                  simpl in H3.  apply andb_prop in H4. apply andb_prop in H1.  destruct H4, H1. destruct n. simpl in H1. apply Z.ltb_lt in H1. apply Zle_bool_imp_le in H4. lia. discriminate. simpl in H1. discriminate.     
 Qed.
 
-  End Specifications.
-
-  
+End Specifications.
